LeanCodePrompts/Utils.lean
@@ -16,3 +16,28 @@ partial def showSyntax : Syntax → String
 | Lean.Syntax.atom _ val => val
 | Lean.Syntax.ident _ _ val _ => val.toString
 | _ => ""
+
+namespace Lean.Json
+
+def parseArrIO (s : String) : IO <| Array Json := do
+  IO.ofExcept $ Json.parse s >>= Json.getArr?
+
+def parseFile (path : System.FilePath) : IO <| Array Json :=
+  IO.FS.readFile path >>= Json.parseArrIO
+
+instance : GetElem Json String Json (λ j k => Except.toBool <| j.getObjVal? k) where
+  getElem := λ j key h =>
+    match j.getObjVal? key, h with
+      | .ok j, _ => j
+      | .error _, h => by simp [Except.toBool] at h
+
+instance : GetElem Json Nat Json (λ j n => Except.toBool <| j.getArrVal? n) where
+  getElem := λ j n h =>
+    match j.getArrVal? n, h with
+      | .ok j, _ => j
+      | .error _, h => by simp [Except.toBool] at h
+
+def getStr! (j : Json) : String :=
+  j.getStr?.toOption.get!
+
+end Lean.Json
