LeanCodePrompts/TeXToUnicodeExamples.lean
@@ -4,5 +4,8 @@ open Lean
 
 def egTeX := "A formula is $\\alpha \\to \\beta := \\unknown$"
 
-#eval teXToUnicode egTeX 
+#eval teXToUnicode egTeX
 
+def egTeX' := "A formula is $a = b$ and $c = d$, also $$X = Y$$ and $b$ = $c$ in $$1 = 2$$."
+
+#eval translateTeX egTeX'
